SyBlocToObc/Correctness.v
@@ -1,6 +1,7 @@
 Require Import Velus.Common.
 Require Import Velus.Operators.
 Require Import Velus.Clocks.
+Require Import Velus.RMemory.
 
 Require Import Velus.NLustre.NLExprSyntax.
 Require Import Velus.NLustre.Stream.
@@ -16,7 +17,8 @@ Require Import Velus.SyBlocToObc.Translation.
 Require Import List.
 Import List.ListNotations.
 
-Open Scope positive.
+(* Open Scope positive. *)
+Open Scope nat.
 Open Scope list.
 
 Module Type CORRECTNESS
@@ -33,5 +35,344 @@ Module Type CORRECTNESS
        (Import SemObc  : OBCSEMANTICS    Ids Op OpAux                    SynObc)
        (Import Trans   : TRANSLATION     Ids Op OpAux Clks ExprSyn SynSB SynObc).
 
+  Definition compat_env (R: env) (mems: PS.t) (me: menv) (ve: venv) :=
+    forall x c,
+      Env.find x R = Some (present c) ->
+      if PS.mem x mems
+      then find_val x me = Some c
+      else Env.find x ve = Some c.
+
+  Section BuildMemWith.
+
+    Context {A B V: Type}.
+    Variable f: A -> V.
+    Variable g: B -> memory V.
+
+    Definition build_mem_with (xs: list (ident * A)) (ys: list (ident * B)) (m: memory V): memory V :=
+      let (xs, vs) := split xs in
+      let (ys, ws) := split ys in
+      Mem (Env.adds xs (map f vs) (values m)) (Env.adds ys (map g ws) (instances m)).
+
+    Lemma build_mem_with_values:
+      forall xs ys m,
+        values (build_mem_with xs ys m) =
+        let (xs, vs) := split xs in
+        Env.adds xs (map f vs) (values m).
+    Proof.
+      intros; unfold build_mem_with; destruct (split xs), (split ys); auto.
+    Qed.
+
+    Lemma build_mem_with_instances:
+      forall xs ys m,
+        instances (build_mem_with xs ys m) =
+        let (ys, ws) := split ys in
+        Env.adds ys (map g ws) (instances m).
+    Proof.
+      intros; unfold build_mem_with; destruct (split xs), (split ys); auto.
+    Qed.
+
+    (* Definition build_mem_with (xs: list (ident * A)) (ys: list (ident * B)) (m: memory V): memory V := *)
+    (*   fold_left (fun m x => add_inst (fst x) (f (snd x)) m) xs *)
+    (*             (fold_left (fun m y => add_val (fst y) (g (snd y)) m) ys m). *)
+
+  End BuildMemWith.
+
+
+  Fixpoint reset_state (P: SynSB.program) (b: ident) : state :=
+    match P with
+    | [] => empty_memory _
+    | bl :: P =>
+      if ident_eqb (b_name bl) b
+      then build_mem_with sem_const (reset_state P) (b_lasts bl) (b_blocks bl) (empty_memory _)
+      else reset_state P b
+    end.
+
+  Lemma reset_state_find_Some:
+    forall P b P' bl,
+      find_block b P = Some (bl, P') ->
+      reset_state P b = build_mem_with sem_const (reset_state P') (b_lasts bl) (b_blocks bl) (empty_memory _).
+  Proof.
+    intros ** Find.
+    induction P as [|bl'].
+    - inv Find.
+    - simpl in *.
+      destruct (ident_eqb (b_name bl') b); auto.
+      inv Find; auto.
+  Qed.
+
+  Lemma reset_state_find_None:
+    forall P b,
+      find_block b P = None ->
+      reset_state P b = empty_memory _.
+  Proof.
+    intros ** Find.
+    induction P as [|bl']; simpl in *; auto.
+    destruct (ident_eqb (b_name bl') b); try discriminate; auto.
+  Qed.
+
+  Lemma find_val_reset_state:
+    forall P b bl P',
+      find_block b P = Some (bl, P') ->
+      (forall x c,
+          In (x, c) (b_lasts bl) ->
+          find_val x (reset_state P b) = Some (sem_const c))
+      /\
+      forall x v,
+        find_val x (reset_state P b) = Some v ->
+        exists c, v = sem_const c /\ In (x, c) (b_lasts bl).
+  Proof.
+    intros.
+    unfold find_val.
+    erewrite reset_state_find_Some; eauto.
+    rewrite build_mem_with_values.
+    pose proof (b_nodup_lasts_blocks bl) as NoDup.
+    apply NoDup_app_weaken in NoDup.
+    induction (b_lasts bl) as [|(x', c')]; simpl.
+    - rewrite Env.adds_nil_nil; setoid_rewrite Env.gempty.
+      split; [contradiction | discriminate].
+    - destruct (split l); simpl.
+      inversion_clear NoDup as [|?? Notin].
+      split; [intros ** [Eq|?]|intros ** Find].
+      + inv Eq; apply Env.find_gsss.
+      + rewrite Env.find_gsso; auto.
+        * now apply IHl.
+        * intro; subst; apply Notin.
+          apply in_map_iff; exists (x', c); auto.
+      + destruct (ident_eq_dec x x').
+        * subst; rewrite Env.find_gsss in Find; inv Find; eauto.
+        * rewrite Env.find_gsso in Find; auto.
+          apply IHl in Find as (?&?&?); eauto.
+  Qed.
+
+  Lemma reset_state_other:
+    forall P P' b bl,
+      find_block b P = None ->
+      b <> b_name bl ->
+      reset_state (P ++ bl :: P') b = reset_state P' b.
+  Proof.
+    intros.
+    destruct (find_block b P') as [[]|] eqn: Find.
+    - symmetry; erewrite reset_state_find_Some; eauto.
+      erewrite <-find_block_other_app in Find; eauto.
+      erewrite reset_state_find_Some; eauto.
+    - symmetry; rewrite reset_state_find_None; auto.
+      rewrite <-find_block_other_app with (P := P) (bl := bl) in Find; eauto.
+      rewrite reset_state_find_None; auto.
+  Qed.
+
+  Lemma initial_reset_state:
+    forall P b P' bl,
+      Ordered_blocks P ->
+      find_block b P = Some (bl, P') ->
+      initial_state P b (reset_state P b).
+  Proof.
+    induction P; try now inversion 1.
+    intros ** Ord Find.
+    econstructor; eauto.
+    - split; eapply find_val_reset_state; eauto.
+    - intros.
+      unfold sub_inst, find_inst.
+      erewrite reset_state_find_Some; eauto.
+      rewrite build_mem_with_instances.
+      pose proof (b_nodup_lasts_blocks bl) as NoDup.
+      apply NoDup_comm, NoDup_app_weaken in NoDup.
+      destruct (split (b_blocks bl)) as (l, l') eqn: Eq.
+      simpl.
+      exists (reset_state P' b'); split.
+      + apply Environment.Env.In_find_adds.
+        * assert (l = map fst (b_blocks bl)) as -> by (now rewrite <-split_fst_map, Eq); auto.
+        * rewrite combine_map_snd.
+          apply in_map_iff.
+          exists (x, b'); split; auto.
+          pose proof (split_combine (b_blocks bl)) as Eq'.
+          rewrite Eq in Eq';  setoid_rewrite Eq'; auto.
+      + simpl in Find.
+        destruct (ident_eqb (b_name a) b) eqn: E.
+        * inv Find.
+          pose proof Ord as Ord'.
+          inversion_clear Ord as [|??? Blocks].
+          eapply Forall_forall in Blocks as (?&?&?&Find'); eauto.
+          apply IHP in Find'; auto.
+          rewrite <-initial_state_tail; auto.
+        *{ pose proof Ord as Ord'.
+           inversion_clear Ord as [|?? Ord'' Blocks]; clear Blocks.
+           rewrite <-initial_state_tail; auto.
+           - apply find_block_app in Find as (P1 & HP &?).
+             rewrite HP in *.
+             apply Ordered_blocks_split in Ord''.
+             eapply Forall_forall in Ord'' as (?&?&?&?& Find'); eauto.
+             simpl in *.
+             rewrite <-find_block_other_app with (P := P1) (bl := bl) in Find'; auto.
+             inversion_clear Ord'.
+             apply IHP in Find'; auto.
+             rewrite reset_state_other in Find'; auto.
+           - admit.
+         }
+  Qed.
+
+
+  Lemma fuu:
+    forall P b P' prog me bl,
+      find_block b P = Some (bl, P') ->
+      exists me',
+        stmt_eval prog me vempty (translate_reset_eqns bl) (me', vempty)
+        /\ initial_state P b me'.
+  Proof.
+    intros.
+    eexists; split.
+    - unfold translate_reset_eqns. reset_method; simpl.
+
+
+
+  Lemma call_reset:
+    forall P b me bl P',
+      find_block b P = Some (bl, P') ->
+      exists me',
+        stmt_call_eval (translate P) me b reset [] me' []
+        /\ initial_state P b me'.
+  Proof.
+    intros ** Find.
+    apply find_block_translate in Find as (?&?&?&?).
+    eexists; split.
+    - econstructor; eauto.
+      + subst; apply exists_reset_method.
+      + rewrite Env.adds_nil_nil. SearchAbout Env.adds nil. SearchAbout find_method reset.
+  Admitted.
+
+  Section BaseTrue.
+
+    Variable (R: env) (mems: PS.t).
+    Variable (me: menv) (ve: venv).
+
+    Lemma typeof_correct:
+      forall e, typeof (translate_lexp mems e) = ExprSyn.typeof e.
+    Proof.
+      induction e; simpl; auto.
+      destruct (PS.mem i mems); auto.
+    Qed.
+
+    Hypothesis Compat_env: compat_env R mems me ve.
+
+    Lemma lexp_correct:
+      forall e c,
+        sem_lexp_instant true R e (present c) ->
+        exp_eval me ve (translate_lexp mems e) c.
+    Proof.
+      induction e;
+        inversion_clear 1 as [|??? Hvar| | | | | | |]; simpl; auto.
+      - constructor; congruence.
+      - apply Compat_env in Hvar.
+        destruct (PS.mem i mems); eauto using exp_eval.
+      - econstructor; eauto.
+        now rewrite typeof_correct.
+      - econstructor; eauto.
+        now rewrite 2 typeof_correct.
+    Qed.
+    Hint Resolve lexp_correct.
+
+    Corollary lexps_correct:
+      forall es cs,
+        sem_lexps_instant true R es (map present cs) ->
+        Forall2 (exp_eval me ve) (map (translate_lexp mems) es) cs.
+    Proof.
+      setoid_rewrite Forall2_map_1; setoid_rewrite Forall2_map_2;
+        intros; eapply Forall2_impl_In; eauto; auto.
+    Qed.
+    Hint Resolve lexps_correct.
+
+    Lemma cexp_correct:
+      forall e c prog x,
+        sem_cexp_instant true R e (present c) ->
+        stmt_eval prog me ve (translate_cexp mems x e) (me, Env.add x c ve).
+    Proof.
+      induction e;
+        inversion 1 as [???? Hvar|???? Hvar| | | |];
+        subst; simpl; eauto.
+      - apply Compat_env in Hvar.
+        econstructor; eauto.
+        + unfold bool_var, tovar.
+          destruct (PS.mem i mems); eauto using exp_eval.
+        + apply val_to_bool_true.
+        + simpl; auto.
+      - apply Compat_env in Hvar.
+        econstructor; eauto.
+        + unfold bool_var, tovar.
+          destruct (PS.mem i mems); eauto using exp_eval.
+        + apply val_to_bool_false.
+        + simpl; auto.
+      - econstructor; eauto.
+        destruct b; match goal with H: present _ = present _ |- _ => inv H end; auto.
+    Qed.
+    Hint Resolve cexp_correct.
+
+    Lemma stmt_eval_Control:
+      forall ck prog s,
+        (sem_clock_instant true R ck false ->
+         stmt_eval prog me ve (Control mems ck s) (me, ve))
+        /\
+        (forall me' ve',
+            sem_clock_instant true R ck true ->
+            stmt_eval prog me ve s (me', ve') ->
+            stmt_eval prog me ve (Control mems ck s) (me', ve')).
+    Proof.
+      induction ck; split;
+        inversion_clear 1 as [ |????? Hvar| |????? Hvar]; simpl; auto.
+      - destruct b; edestruct IHck; eauto.
+      - apply Compat_env in Hvar.
+        unfold bool_var, tovar.
+        destruct b0; simpl;
+          destruct (PS.mem i mems); eapply IHck; eauto using stmt_eval, exp_eval.
+      - apply Compat_env in Hvar.
+        unfold bool_var, tovar.
+        intros; destruct b;
+          destruct (PS.mem i mems); eapply IHck; eauto using stmt_eval, exp_eval.
+    Qed.
+
+    Corollary stmt_eval_Control_absent:
+      forall ck prog s,
+        sem_clock_instant true R ck false ->
+        stmt_eval prog me ve (Control mems ck s) (me, ve).
+    Proof. apply stmt_eval_Control. Qed.
+
+    Corollary stmt_eval_Control_present:
+      forall ck prog s me' ve',
+        sem_clock_instant true R ck true ->
+        stmt_eval prog me ve s (me', ve') ->
+        stmt_eval prog me ve (Control mems ck s) (me', ve').
+    Proof. apply stmt_eval_Control. Qed.
+
+    Lemma foo:
+      forall P S I S' eq,
+        sem_equation P true R S I S' eq ->
+        exists me' ve',
+          stmt_eval (translate P) me ve (translate_eqn mems eq) (me', ve').
+    Proof.
+      destruct eq;
+        inversion_clear 1 as [????????? Hexp|
+                              ???????????? Hexp|
+                              ????????????? Init|
+                              ???????????????? Hexps]; simpl.
+      - inv Hexp;
+          eauto using stmt_eval_Control_absent, stmt_eval_Control_present, cexp_correct.
+      - inv Hexp;
+          eauto 6 using stmt_eval_Control_absent, stmt_eval_Control_present, stmt_eval.
+      - destruct r; eauto using stmt_eval_Control_absent.
+        inversion_clear Init as [???? Find Rst].
+        apply find_block_translate in Find as (?&?&?&?).
+        admit.
+        (* do 2 eexists. *)
+        (* apply stmt_eval_Control_present; auto. *)
+        (* econstructor; eauto. *)
+
+        (* econstructor; eauto. *)
+        (* + subst; apply exists_reset_method. *)
+      - inv Hexps; eauto using stmt_eval_Control_absent.
+        admit.
+        (* do 2 eexists. *)
+        (* apply stmt_eval_Control_present; auto. *)
+        (* econstructor; eauto. *)
+    Qed.
+
+  End BaseTrue.
 
 End CORRECTNESS.
